src/impl/TLS13.Impl.Server.Driver.BufferedClose.fst
@@ -142,29 +142,6 @@ fn abort_connected
   TLS13.Impl.Server.Driver.BufferedTransport.close_transport_once d
 }
 
-fn abort
-  (d:DS.top_server_driver)
-  (wire_received:Ghost.erased B.bytes)
-  (wire_sent:Ghost.erased B.bytes)
-  (pending:Ghost.erased B.bytes)
-  (app_log:Ghost.erased (CI.application_log B.bytes))
-  requires
-    DS.top_server_channel_inv
-      d
-      (Ghost.reveal wire_received)
-      (Ghost.reveal wire_sent)
-      (Ghost.reveal pending)
-      (Ghost.reveal app_log)
-  ensures
-    exists* st certificate_chain credential_identity.
-      DS.top_server_driver_closed
-        d st certificate_chain credential_identity
-{
-  BC.open_channel_invariant
-    d wire_received wire_sent pending app_log;
-  abort_connected d
-}
-
 fn abort_terminal
   (d:DS.top_server_driver)
   (wire_received:Ghost.erased B.bytes)
